compiler/src/FlatToRiscvLiterals.v
@@ -104,12 +104,12 @@ Section FlatToRiscvLiterals.
            end.
 
   Lemma compile_lit_correct_full: forall (initialL: RiscvMachineL) post x v R,
-      initialL.(getNextPc) = add initialL.(getPc) (ZToReg 4) ->
+      initialL.(getNextPc) = add initialL.(getPc) (word.of_Z 4) ->
       let insts := compile_stmt (FlatImp.SLit x v) in
-      let d := mul (ZToReg 4) (ZToReg (Zlength insts)) in
+      let d := mul (word.of_Z 4) (word.of_Z (Z.of_nat (List.length insts))) in
       (program initialL.(getPc) insts * R)%sep initialL.(getMem) ->
       valid_registers (FlatImp.SLit x v) ->
-      runsTo (withRegs (map.put initialL.(getRegs) x (ZToReg v))
+      runsTo (withRegs (map.put initialL.(getRegs) x (word.of_Z v))
              (withPc     (add initialL.(getPc) d)
              (withNextPc (add initialL.(getNextPc) d)
              (withMetrics (updateMetricsForLiteral v initialL.(getMetrics)) initialL))))
@@ -138,7 +138,7 @@ Section FlatToRiscvLiterals.
       simpl in P.
       run1det. run1det.
       match_apply_runsTo.
-      simpl_MetricRiscvMachine_get_set. f_equal; [|solve_MetricLog].
+      f_equal; [|solve_MetricLog].
       f_equal.
       + rewrite map.put_put_same. f_equal.
         apply word.signed_inj.
@@ -184,16 +184,17 @@ Section FlatToRiscvLiterals.
       end.
       cbv [List.app program array] in P.
       simpl in *. (* if you don't remember enough values, this might take forever *)
-      autorewrite with rew_Zlength in N.
-      simpl in N.
-      run1det. simpl_MetricRiscvMachine_get_set. repeat unfold_MetricLog.
-      run1det. simpl_MetricRiscvMachine_get_set. repeat unfold_MetricLog.
-      run1det. simpl_MetricRiscvMachine_get_set. repeat unfold_MetricLog.
-      run1det. simpl_MetricRiscvMachine_get_set. repeat unfold_MetricLog.
-      run1det. simpl_MetricRiscvMachine_get_set. repeat unfold_MetricLog.
-      run1det. simpl_MetricRiscvMachine_get_set. repeat unfold_MetricLog.
-      run1det. simpl_MetricRiscvMachine_get_set. repeat unfold_MetricLog.
-      run1det. simpl_MetricRiscvMachine_get_set. repeat unfold_MetricLog.
+      repeat match type of X with
+             | _ /\ _ => destruct X as [? X]
+             end.
+      run1det. repeat unfold_MetricLog.
+      run1det. repeat unfold_MetricLog.
+      run1det. repeat unfold_MetricLog.
+      run1det. repeat unfold_MetricLog.
+      run1det. repeat unfold_MetricLog.
+      run1det. repeat unfold_MetricLog.
+      run1det. repeat unfold_MetricLog.
+      run1det. repeat unfold_MetricLog.
       match_apply_runsTo.
       f_equal; [|simpl; solve_MetricLog].
       f_equal.
